WIP on SpecWithAPI

src/Protocols/SigmaKeyExchange/Combinators.v
@@ -2,8 +2,9 @@ Require Import Coq.Lists.List.
 
 Create HintDb trace_combinators discriminated.
 
-Fixpoint holds_of_messages_around_nth_message_matching_aux
-         (n : nat)
+Fixpoint holds_of_messages_around_nth_messages_matching_aux
+         (is_n : nat -> Prop)
+         (if_none_found : Prop)
          {T}
          (matcher : T -> Prop)
          (property : list T -> T -> list T -> Prop)
@@ -11,63 +12,111 @@ Fixpoint holds_of_messages_around_nth_message_matching_aux
          (trace : list T)
 : Prop
 := match trace with
-   | nil => True
+   | nil => if_none_found
    | m :: ms
      => (matcher m ->
-         match n with
-         | 0 => property pre_trace m ms
-         | S n'
-           => holds_of_messages_around_nth_message_matching_aux
-                n'
-                matcher
-                property
-                (pre_trace ++ m::nil)
-                ms
-         end)
+         (is_n 0 -> property pre_trace m ms)
+         /\ holds_of_messages_around_nth_messages_matching_aux
+              (fun n' => is_n (S n'))
+              (is_n 0 \/ if_none_found)
+              matcher
+              property
+              (pre_trace ++ m::nil)
+              ms)
         /\ (~matcher m
-            -> holds_of_messages_around_nth_message_matching_aux
-                 n
+            -> holds_of_messages_around_nth_messages_matching_aux
+                 is_n
+                 if_none_found
                  matcher property (pre_trace ++ (m::nil)) ms)
    end%list.
-Fixpoint holds_of_messages_around_nth_message_matching
-         (n : nat)
-         {T}
-         (matcher : T -> Prop)
-         (property : list T -> T -> list T -> Prop)
-         (trace : list T)
+Class reverse_search := do_reverse : bool.
+Definition holds_of_messages_around_nth_messages_matching
+           {rev : reverse_search}
+           (is_n : nat -> Prop)
+           (if_none_found : Prop)
+           {T}
+           (matcher : T -> Prop)
+           (property : list T -> T -> list T -> Prop)
+           (trace : list T)
   : Prop
-  := holds_of_messages_around_nth_message_matching_aux
-       n matcher property nil trace.
-Definition holds_of_messages_before_nth_message_matching
-           (n : nat)
+  := holds_of_messages_around_nth_messages_matching_aux
+       is_n if_none_found
+       matcher
+       (fun pre m post
+        => if rev
+           then property (List.rev post) m (List.rev pre)
+           else property pre m post)
+       nil
+       (if rev then List.rev trace else trace).
+Hint Unfold holds_of_messages_around_nth_messages_matching : trace_combinators.
+Notation holds_of_messages_around_nth_message_matching n
+  := (holds_of_messages_around_nth_messages_matching (fun n' => n = n') True).
+Definition holds_of_messages_before_nth_messages_matching
+           {rev : reverse_search}
+           (is_n : nat -> Prop)
+           (if_none_found : Prop)
            {T}
            (matcher : T -> Prop)
            (property : list T -> T -> Prop)
            (trace : list T)
   : Prop
-  := holds_of_messages_around_nth_message_matching
-       n matcher (fun before m after => property before m) trace.
-Hint Unfold holds_of_messages_before_nth_message_matching : trace_combinators.
-Definition holds_of_nth_message_matching
-           (n : nat)
+  := holds_of_messages_around_nth_messages_matching
+       is_n if_none_found matcher (fun before m after => property before m) trace.
+Hint Unfold holds_of_messages_before_nth_messages_matching : trace_combinators.
+Notation holds_of_messages_before_nth_message_matching n
+  := (holds_of_messages_before_nth_messages_matching (fun n' => n = n') True).
+Notation holds_of_messages_before_all_messages_matching
+  := (holds_of_messages_before_nth_messages_matching (fun _ => True) True).
+Definition holds_of_nth_messages_matching
+           {rev : reverse_search}
+           (is_n : nat -> Prop)
+           (if_none_found : Prop)
            {T}
            (matcher : T -> Prop)
            (property : T -> Prop)
            (trace : list T)
   : Prop
-  := holds_of_messages_around_nth_message_matching
-       n matcher (fun _ m _=> property m) trace.
+  := holds_of_messages_around_nth_messages_matching
+       is_n if_none_found matcher (fun _ m _=> property m) trace.
+Hint Unfold holds_of_nth_messages_matching : trace_combinators.
+Definition holds_of_nth_messages_matching_if_they_exist {rev} is_n {T}
+  := holds_of_nth_messages_matching (rev:=rev) is_n True (T:=T).
+Hint Unfold holds_of_nth_messages_matching_if_they_exist : trace_combinators.
+Definition holds_of_nth_message_matching {rev} n {T}
+  := @holds_of_nth_messages_matching rev (fun n' => n = n') True T.
 Hint Unfold holds_of_nth_message_matching : trace_combinators.
-Definition holds_of_messages_after_nth_message_matching
-           (n : nat)
+Definition holds_of_nth_to_last_message_matching n {T}
+  := holds_of_nth_message_matching n (rev:=true) (T:=T).
+Hint Unfold holds_of_nth_to_last_message_matching : trace_combinators.
+Definition holds_of_all_messages_matching {T}
+  := @holds_of_nth_messages_matching false (fun _ => True) True T.
+Hint Unfold holds_of_all_messages_matching : trace_combinators.
+Definition holds_of_all_messages {T}
+  := @holds_of_all_messages_matching T (fun _ => True).
+Hint Unfold holds_of_all_messages : trace_combinators.
+Definition holds_of_nth_message_matching_which_must_exist {rev} n {T}
+  := @holds_of_nth_messages_matching rev (fun n' => n = n') False T.
+Hint Unfold holds_of_nth_message_matching_which_must_exist : trace_combinators.
+Definition holds_of_nth_to_last_message_matching_which_must_exist n {T}
+  := holds_of_nth_message_matching_which_must_exist n (rev:=true) (T:=T).
+Hint Unfold holds_of_nth_to_last_message_matching_which_must_exist : trace_combinators.
+Definition nth_message_matching_exists {rev} n {T} matcher
+  := @holds_of_nth_message_matching_which_must_exist rev n T matcher (fun _ => True).
+Hint Unfold nth_message_matching_exists : trace_combinators.
+Definition holds_of_messages_after_nth_messages_matching
+           {rev : reverse_search}
+           (is_n : nat -> Prop)
+           (if_none_found : Prop)
            {T}
            (matcher : T -> Prop)
            (property : T -> list T -> Prop)
            (trace : list T)
   : Prop
-  := holds_of_messages_around_nth_message_matching
-       n matcher (fun before m after => property m after) trace.
-Hint Unfold holds_of_messages_after_nth_message_matching : trace_combinators.
+  := holds_of_messages_around_nth_messages_matching
+       is_n if_none_found matcher (fun before m after => property m after) trace.
+Hint Unfold holds_of_messages_after_nth_messages_matching : trace_combinators.
+Notation holds_of_messages_after_nth_message_matching n
+  := (holds_of_messages_after_nth_messages_matching (fun n' => n = n') True).
 Definition on_input {input output T} (f : input -> T) : input * output -> T
   := fun '(i, o) => f i.
 Hint Unfold on_input : trace_combinators.
@@ -75,41 +124,57 @@ Definition on_output {input output T} (f : output -> T) : input * output -> T
   := fun '(i, o) => f o.
 Hint Unfold on_output : trace_combinators.
 
-Definition holds_of_all_messages_after_nth_message_matching_gen
+Definition holds_of_all_messages_after_nth_messages_matching_gen
+           {rev : reverse_search}
            (include_nth_msg : bool)
-           (n : nat)
+           (is_n : nat -> Prop)
+           (if_none_found : Prop)
            {T}
            (matcher : T -> Prop)
            (property : T (* nth_msg *) -> T (* other message *) -> Prop)
            (trace : list T)
   : Prop
-  := holds_of_messages_after_nth_message_matching
-       n
+  := holds_of_messages_after_nth_messages_matching
+       is_n
+       if_none_found
        matcher
        (fun m after
         => List.Forall (property m) (if include_nth_msg then m::after else after))
        trace.
-Hint Unfold holds_of_all_messages_after_nth_message_matching_gen : trace_combinators.
-Notation holds_of_all_messages_after_nth_message_matching
-  := (holds_of_all_messages_after_nth_message_matching_gen true).
-Notation holds_of_all_messages_strictly_after_nth_message_matching
-  := (holds_of_all_messages_after_nth_message_matching_gen false).
-Definition holds_of_some_message_before_nth_message_matching_gen
+Hint Unfold holds_of_all_messages_after_nth_messages_matching_gen : trace_combinators.
+Notation holds_of_all_messages_after_nth_messages_matching
+  := (holds_of_all_messages_after_nth_messages_matching_gen true).
+Notation holds_of_all_messages_after_nth_message_matching n
+  := (holds_of_all_messages_after_nth_messages_matching (fun n' => n = n') True).
+Notation holds_of_all_messages_strictly_after_nth_messages_matching
+  := (holds_of_all_messages_after_nth_messages_matching_gen false).
+Notation holds_of_all_messages_strictly_after_nth_message_matching n
+  := (holds_of_all_messages_strictly_after_nth_messages_matching (fun n' => n = n') True).
+Definition holds_of_some_message_before_nth_messages_matching_gen
+           {rev : reverse_search}
            (include_nth_message : bool)
-           (n : nat)
+           (is_n : nat -> Prop)
+           (if_none_found : Prop)
            {T}
            (matcher : T -> Prop)
            (property : T (* nth_msg *) -> T (* other message *) -> Prop)
            (trace : list T)
   : Prop
-  := holds_of_messages_before_nth_message_matching
-       n
+  := holds_of_messages_before_nth_messages_matching
+       is_n
+       if_none_found
        matcher
        (fun before m
         => List.Exists (property m) (if include_nth_message then (before ++ (m::nil))%list else before))
        trace.
-Hint Unfold holds_of_some_message_before_nth_message_matching_gen : trace_combinators.
-Notation holds_of_some_message_before_nth_message_matching
-  := (holds_of_some_message_before_nth_message_matching_gen true).
-Notation holds_of_some_message_strictly_before_nth_message_matching
-  := (holds_of_some_message_before_nth_message_matching_gen false).
+Hint Unfold holds_of_some_message_before_nth_messages_matching_gen : trace_combinators.
+Notation holds_of_some_message_before_nth_messages_matching
+  := (holds_of_some_message_before_nth_messages_matching_gen true).
+Notation holds_of_some_message_before_nth_message_matching n
+  := (holds_of_some_message_before_nth_messages_matching (fun n' => n = n') True).
+Notation holds_of_some_message_strictly_before_nth_messages_matching
+  := (holds_of_some_message_before_nth_messages_matching_gen false).
+Notation holds_of_some_message_strictly_before_nth_message_matching n
+  := (holds_of_some_message_strictly_before_nth_messages_matching (fun n' => n = n') True).
+
+Global Instance default_rev : reverse_search := false.
