src/Protocols/SigmaKeyExchange/SpecWithAPI.v
@@ -1,0 +1,731 @@
+Require Import Crypto.Spec.Trace.
+Require Import Crypto.Protocols.SigmaKeyExchange.Combinators.
+(**
+// All single-letter symbols in this comment represent public DH keys.
+// Capital letters represent long-term and others are per-connection
+// ephemeral. [msg](PK1<>PK2) denotes nacl/box authenticated encryption.
+//--> a
+//<-- b
+//<-- [B,[b,a](B<>a)](a<>b)
+//--> [A,[a,b](A<>b)](a<>b)
+//--> [data](a<>b)
+//<-- [data](a<>b)
+*)
+
+(* Parameter: g *)
+(* Per-connection parameter: A *)
+(* Per-connection choice: x *)
+(* Per-connection choice: b *)
+(* Per-connection choice: B *)
+(* Constraint: if there's a first message on the wire from our side,
+then there must be a message from the RNG before that which gives x *)
+(* Constraint: if there's a first message on the wire from our side, it
+must be g^x *)
+(* Constraint: if you recieve more than just [b] before you send [a],
+must abort *)
+(* Constraint: if you send a non-abort message after sending [a], you
+must have recieved [b] (and it must match the choice of [b]) *)
+(* Constraint: the form of our second message must be correct *)
+(* Constraint: if you send a non-abort message after sending [a] and
+"the long message", you must have recieved a long message, and it must
+be the message you got immediately after the short message, and it
+must match the choice of [B], and the format must be correct *)
+
+(* Secrets constraint: If you recieve a randomness message, you may
+immediately emit [g^x] and update the secret-x-value with [x], or you
+may do anything which does not depend on the contents of the random
+message.  (the decision must depend only on public things) *)
+(* Secrets constraint: You may at any time emit a message matching
+long-form or short-form using the secret-x-value in the appropriate
+place and not in other places, or else you must emit somthing not
+depending on the secret-x-value (the decision must depend only on
+public things) *)
+
+Section spec.
+  Context (connection_id : Type)
+          (secret public : Type)
+          (message ciphertext : Type)
+          (text_of_pair : message * message -> message)
+          (text_of_public : public -> message)
+          (text_of_cipher : ciphertext -> message)
+          (pair_of_text : message -> message * message)
+          (public_of_text : message -> public)
+          (cipher_of_text : message -> ciphertext).
+  Let random := secret.
+  Context (keygen : secret -> public) (* Parameter: g *)
+          (box_seal : secret -> public -> message -> ciphertext)
+          (box_open : secret -> public -> ciphertext -> option message).
+
+  Section per_connection_parameters.
+    Context (our_longterm_secret : secret).
+    Let our_longterm_public : public (* Per-connection parameter: A *)
+      := keygen our_longterm_secret.
+    Section per_connection_choices.
+      Context (our_ephemeral_secret : secret) (* Per-connection choice: x *)
+              (their_ephemeral_public : public) (* Per-connection choice: b *)
+              (their_longterm_public : public) (* Per-connection choice: B *).
+      Let our_ephemeral_public : public
+        := keygen our_ephemeral_secret.
+
+      Context {state : Type}.
+
+      Inductive input :=
+      | Random (_ : random) | ConnectionStart | RecieveNetwork (_ : message)
+      | APISendNetwork | APICloseConnection | APIUserOutput.
+
+      Inductive pre_output :=
+      | RequestRandom | SendNetwork (_ : message) | CloseConnection | UserOutput (_ : secret * public * public)
+      | APIGotRandom | APIGotConnectionStart
+      | APIGotTheirEphemeralPublic (_ : message) (_ : public)
+      | APIGotTheirLongtermPublicAndPassedValidation (_ : message) (_ : public)
+      | APIGotTheirLongformFailedValidation (_ : message)
+      | APIGotRecieveNetworkGeneric (_ : message).
+      Let output := option pre_output.
+
+      (* Constraint: we don't send anything after CloseConnection *)
+      Definition close_connection_closed
+                 (trace : list (input * output)) : Prop
+        := holds_of_all_messages_strictly_after_nth_message_matching
+             0
+             (on_output (fun m_out => m_out = Some CloseConnection))
+             (fun _ => on_output (fun m_out => m_out = None))
+             trace.
+
+      (* Constraint: if there's a first message on the wire from our
+          side, then there must be a message from the RNG before that
+          which gives x *)
+      Definition get_randomness_spec
+                 (trace : list (input * output)) : Prop
+        := holds_of_some_message_before_nth_message_matching
+             0
+             (on_output (fun m_out => exists v, m_out = Some (SendNetwork v)))
+             (fun _ => on_input (fun m_in => m_in = Random our_ephemeral_secret))
+             trace.
+
+      Let Send_a := Some (SendNetwork (text_of_public our_ephemeral_public)).
+
+      (* Constraint: if there's a first message on the wire from our
+          side, it must be g^x *)
+      Definition output_g_x
+                 (trace : list (input * output)) : Prop
+        := holds_of_nth_message_matching
+             0
+             (on_output (fun m_out => exists v, m_out = Some (SendNetwork v)))
+             (on_output (fun m_out => m_out = Send_a))
+             trace.
+
+      (* Constraint: if you recieve more than just [b] before you send
+          [a], must abort *)
+      (* Skipped for now *)
+
+      (* Constraint: if you send a non-abort message after sending
+          [a], you must have recieved [b] (and it must match the
+          choice of [b]) *)
+      Definition must_set_b
+                 (trace : list (input * output)) : Prop
+        := nth_message_matching_exists
+             1
+             (on_output (fun m_out => exists v, m_out = Some (SendNetwork v)))
+             trace
+           -> holds_of_nth_message_matching
+                0
+                (on_input (fun m_in => exists v, m_in = RecieveNetwork v))
+                (on_input (fun m_in => m_in = RecieveNetwork (text_of_public their_ephemeral_public)))
+                trace.
+      Definition must_recieve_b
+                 (trace : list (input * output)) : Prop
+        := holds_of_some_message_strictly_before_nth_message_matching
+             1
+             (on_output (fun m_out => exists v, m_out = Some (SendNetwork v)))
+             (fun _ => on_input (fun m_in => m_in = RecieveNetwork (text_of_public their_ephemeral_public)))
+             trace.
+
+      Let longform
+        := (text_of_cipher
+              (box_seal
+                 our_ephemeral_secret
+                 their_ephemeral_public
+                 (text_of_pair
+                    (text_of_public our_longterm_public,
+                     text_of_cipher
+                       (box_seal
+                          our_longterm_secret
+                          their_ephemeral_public
+                          (text_of_pair
+                             (text_of_public our_ephemeral_public,
+                              text_of_public their_ephemeral_public))))))).
+
+      (* Constraint: the form of our second message must be correct *)
+      (* //--> [A,[a,b](A<>b)](a<>b) *)
+      Definition second_message_correct
+                 (trace : list (input * output)) : Prop
+        := holds_of_nth_message_matching
+             1
+             (on_output (fun m_out => exists v, m_out = Some (SendNetwork v)))
+             (on_output
+                (fun m_out
+                 => m_out
+                    = Some
+                        (SendNetwork
+                           longform)))
+             trace.
+
+      Let input_passes_validation m_in
+        := (forall v boxed_b_a,
+               m_in = RecieveNetwork v
+               -> box_open
+                    our_ephemeral_secret
+                    their_ephemeral_public
+                    (cipher_of_text v)
+                  = Some (text_of_pair
+                            (text_of_public their_longterm_public,
+                             text_of_cipher boxed_b_a))
+                  /\ box_open
+                       our_ephemeral_secret
+                       their_longterm_public
+                       boxed_b_a
+                     = Some (text_of_pair
+                               (text_of_public their_ephemeral_public,
+                                text_of_public our_ephemeral_public))).
+
+      (* Constraint: if you send a non-abort message after sending [a]
+          and "the long message", you must have recieved a long
+          message, and it must be the message you got immediately
+          after the short message, and it must match the choice of
+          [B], and the format must be correct *)
+      (* //<-- [B,[b,a](B<>a)](a<>b) *)
+      Definition second_message_recieved_correct_form
+                 (trace : list (input * output)) : Prop
+        := nth_message_matching_exists
+             2
+             (on_output (fun m_out => exists v, m_out = Some (SendNetwork v)))
+             trace
+           -> holds_of_nth_message_matching
+                1
+                (on_input (fun m_in => exists v, m_in = RecieveNetwork v))
+                (on_input
+                   (fun m_in
+                    => forall v boxed_b_a,
+                        m_in = RecieveNetwork v
+                        -> box_open
+                             our_ephemeral_secret
+                             their_ephemeral_public
+                             (cipher_of_text v)
+                           = Some (text_of_pair
+                                     (text_of_public their_longterm_public,
+                                      text_of_cipher boxed_b_a))
+                           /\ box_open
+                                our_ephemeral_secret
+                                their_longterm_public
+                                boxed_b_a
+                              = Some (text_of_pair
+                                        (text_of_public their_ephemeral_public,
+                                         text_of_public our_ephemeral_public))))
+                trace.
+      (* Also spec output here *)
+      Definition second_message_recieved
+                 (trace : list (input * output)) : Prop
+        := holds_of_some_message_strictly_before_nth_message_matching
+             0
+             (on_output (fun m_out => exists v, m_out = Some (UserOutput v)))
+             (fun _ => on_input input_passes_validation)
+             trace.
+      Definition output_correct_form
+                 (trace : list (input * output)) : Prop
+        := holds_of_nth_message_matching
+             0
+             (on_output (fun m_out => exists v, m_out = Some (UserOutput v)))
+             (on_output
+                (fun m_out
+                 => m_out
+                    = Some
+                        (UserOutput
+                           (our_ephemeral_secret,
+                            their_ephemeral_public,
+                            their_longterm_public))))
+             trace.
+      Definition nothing_after_user_output
+                 (trace : list (input * output)) : Prop
+        := holds_of_all_messages_strictly_after_nth_message_matching
+             0
+             (on_output (fun m_out => exists v, m_out = Some (UserOutput v)))
+             (fun _ => on_output (fun m_out => m_out = None))
+             trace.
+
+      Definition trace_satisfies_external_SKE_spec (trace : list (input * output)) : Prop
+        := close_connection_closed trace
+           /\ get_randomness_spec trace
+           /\ output_g_x trace
+           /\ must_set_b trace
+           /\ must_recieve_b trace
+           /\ second_message_correct trace
+           /\ second_message_recieved_correct_form trace
+           /\ second_message_recieved trace
+           /\ output_correct_form trace
+           /\ nothing_after_user_output trace.
+      Section secrets.
+        Definition on_input_Random
+                   (trace : list (input * output)) : Prop
+          := holds_of_all_messages
+               (fun '(m_in, m_out)
+                => (exists v, m_in = Random v)
+                   <-> m_out = Some APIGotRandom)
+               trace.
+        Definition on_input_ConnectionStart
+                   (trace : list (input * output)) : Prop
+          := holds_of_all_messages
+               (fun '(m_in, m_out)
+                => m_in = ConnectionStart
+                   <-> m_out = Some APIGotConnectionStart)
+               trace.
+        Definition on_output_CloseConnection
+                   (trace : list (input * output)) : Prop
+          := holds_of_all_messages
+               (fun '(m_in, m_out)
+                => m_in = APICloseConnection
+                   <-> m_out = Some CloseConnection)
+               trace.
+        Definition on_output_UserOutput
+                   (trace : list (input * output)) : Prop
+          := holds_of_all_messages
+               (fun '(m_in, m_out)
+                => m_in = APIUserOutput
+                   <-> (exists v, m_out = Some (UserOutput v)))
+               trace.
+        Definition on_output_SendNetwork
+                   (trace : list (input * output)) : Prop
+          := holds_of_all_messages
+               (fun '(m_in, m_out)
+                => m_in = APISendNetwork
+                   <-> (exists v, m_out = Some (SendNetwork v)))
+               trace.
+        Definition on_input_RecieveNetwork
+                   (trace : list (input * output)) : Prop
+          := holds_of_all_messages
+               (fun '(m_in, m_out)
+                => (exists v, m_in = RecieveNetwork v)
+                   <-> match m_in, m_out with
+                       | RecieveNetwork v, Some (APIGotTheirEphemeralPublic v' _)
+                       | RecieveNetwork v, Some (APIGotTheirLongtermPublicAndPassedValidation v' _)
+                       | RecieveNetwork v, Some (APIGotTheirLongformFailedValidation v')
+                       | RecieveNetwork v, Some (APIGotRecieveNetworkGeneric v')
+                         => v = v'
+                       | _, _ => False
+                       end)
+               trace.
+        Definition on_input_RecieveNetwork0
+                   (trace : list (input * output)) : Prop
+          := holds_of_nth_message_matching
+               0
+               (on_input (fun m_in => exists v, m_in = RecieveNetwork v))
+               (fun '(m_in, m_out)
+                => exists v,
+                    m_in = RecieveNetwork v
+                    /\ m_out = Some (APIGotTheirEphemeralPublic v (public_of_text v)))
+               trace.
+        Definition on_input_RecieveNetwork1
+                   (trace : list (input * output)) : Prop
+          := holds_of_nth_message_matching
+               1
+               (on_input (fun m_in => exists v, m_in = RecieveNetwork v))
+               (fun '(m_in, m_out)
+                => exists v,
+                    m_in = RecieveNetwork v
+                    /\ m_out = Some (APIGotTheirEphemeralPublic v (public_of_text v)))
+               trace.
+        Definition on_input_RecieveNetwork2
+                   (trace : list (input * output)) : Prop
+          := holds_of_nth_message_matching
+               2
+               (on_input (fun m_in => exists v, m_in = RecieveNetwork v))
+               (fun '(m_in, m_out)
+                => exists v,
+                    m_in = RecieveNetwork v
+                    /\ ((input_passes_validation m_in
+                         /\ m_out = Some (APIGotTheirLongtermPublicAndPassedValidation v their_longterm_public))
+                        \/ (~input_passes_validation m_in
+                            /\ m_out = Some (APIGotTheirLongformFailedValidation v))))
+               trace.
+        Definition on_input_RecieveNetworkGe3
+                   (trace : list (input * output)) : Prop
+          := holds_of_nth_messages_matching_if_they_exist
+               (fun n => n > 2)
+               (on_input (fun m_in => exists v, m_in = RecieveNetwork v))
+               (fun '(m_in, m_out)
+                => exists v,
+                    m_in = RecieveNetwork v /\ m_out = Some (APIGotRecieveNetworkGeneric v))
+               trace.
+
+        Definition trace_satisfies_full_SKE_spec (trace : list (input * output)) : Prop
+          := trace_satisfies_external_SKE_spec trace
+             /\ on_input_Random trace
+             /\ on_input_ConnectionStart trace
+             /\ on_output_CloseConnection trace
+             /\ on_output_UserOutput trace
+             /\ on_output_SendNetwork trace
+             /\ on_input_RecieveNetwork trace
+             /\ on_input_RecieveNetwork0 trace
+             /\ on_input_RecieveNetwork1 trace
+             /\ on_input_RecieveNetwork2 trace
+             /\ on_input_RecieveNetworkGe3 trace.
+      End secrets.
+
+      Definition at_most_one {T} (P : T -> Prop)
+        := forall x y : T, P x -> P y -> x = y.
+
+      Definition is_deterministicT
+        := forall (partial_trace : list (input * output))
+                  (m_in : input),
+          at_most_one
+            (fun m_out
+             => (exists rest : list (input * output),
+                    trace_satisfies_full_SKE_spec (partial_trace ++ (m_in, m_out)::rest))).
+
+      Require Import Crypto.Util.Tactics.DestructHead.
+      Require Import Crypto.Util.Tactics.Test.
+      Require Import Crypto.Util.Option.
+      Lemma pull_ex_not {T} (P : T -> Prop)
+        : (~ex P) <-> forall v, ~P v.
+      Proof.
+        split; intros H; [ intros v H' | intros [v H'] ];
+          eapply H; [ eexists | ]; eassumption.
+      Qed.
+      Lemma impl_and_l {A B C : Prop} : (A /\ B -> C) <-> (A -> B -> C).
+      Proof. tauto. Qed.
+      Lemma holds_of_messages_around_nth_messages_matching_aux_lift_impl
+            is_n
+            (P1 P2 : Prop)
+            (HP : P1 -> P2)
+            T
+            (matcher : _ -> Prop)
+            (property1 property2 : _ -> _ -> _ -> Prop)
+            init1 init2
+            (Hproperty : forall pre m post, matcher m -> property1 (init1 ++ pre)%list m post -> property2 (init2 ++ pre)%list m post)
+            trace
+        : @holds_of_messages_around_nth_messages_matching_aux is_n P1 T matcher property1 init1 trace
+          -> @holds_of_messages_around_nth_messages_matching_aux is_n P2 T matcher property2 init2 trace.
+      Proof.
+        clear -Hproperty HP.
+        revert P1 P2 HP is_n init1 init2 Hproperty; induction trace as [|x xs IHxs]; intros P1 P2 HP is_n init1 init2 Hproperty; simpl.
+        { assumption. }
+        { pose proof (Hproperty nil).
+          assert (Hp' : forall pre m post,
+                     matcher m
+                     -> property1 ((init1 ++ x::nil) ++ pre)%list m post
+                     -> property2 ((init2 ++ x::nil) ++ pre)%list m post)
+            by (intros ???; rewrite <- !List.app_assoc; apply Hproperty).
+          repeat first [ progress simpl @List.app in *
+                       | progress rewrite !List.app_nil_r in *
+                       | apply conj
+                       | intro
+                       | assumption
+                       | progress destruct_head'_and
+                       | match goal with
+                         | [ H : ?A -> ?B, H' : ?A |- _ ] => specialize (H H')
+                         end
+                       | solve [ eauto ] ].
+          { eapply IHxs; [ .. | eassumption ]; [ tauto | eauto ]. } }
+      Qed.
+      Lemma holds_of_all_messages_cons {T} P x xs
+        : @holds_of_all_messages T P (x :: xs)
+          <-> (P x /\ @holds_of_all_messages T P xs).
+      Proof.
+        clear.
+        repeat autounfold with trace_combinators; simpl.
+        repeat first [ apply conj
+                     | intro
+                     | assumption
+                     | progress destruct_head'_and
+                     | match goal with
+                       | [ H : True -> _ |- _ ] => specialize (H I)
+                       | [ H : ~True -> _ |- _ ] => clear H
+                       end
+                     | solve [ eauto ]
+                     | eapply holds_of_messages_around_nth_messages_matching_aux_lift_impl; [.. | eassumption ] ].
+      Qed.
+      Lemma holds_of_all_messages_app {T} P ls1 ls2
+        : @holds_of_all_messages T P (ls1 ++ ls2)
+          <-> (@holds_of_all_messages T P ls1 /\ @holds_of_all_messages T P ls2).
+      Proof.
+        clear.
+        revert ls2; induction ls1 as [|x xs IHxs]; intro ls2.
+        { repeat autounfold with trace_combinators; simpl; tauto. }
+        { simpl; rewrite !holds_of_all_messages_cons, IHxs; tauto. }
+      Qed.
+      Lemma is_deterministic : is_deterministicT.
+      Proof.
+        intros partial_trace m_in x y [restx Hx] [resty Hy].
+        unfold trace_satisfies_full_SKE_spec in *.
+        unfold on_input_Random, on_input_ConnectionStart, on_output_CloseConnection, on_output_SendNetwork, on_output_UserOutput in *.
+        (*destruct_head'_and
+        , trace_satisfies_external_SKE_spec in *.*)
+        Local Ltac do_unfold :=
+          repeat first [ progress simpl @List.app in *
+                       | match goal with
+                         | [ H : context[?f _ /\ _] |- _ ]
+                           => lazymatch type of f with
+                              | list _ -> _ => unfold f in H
+                              end
+                         | [ H : context[_ /\ ?f _] |- _ ]
+                           => lazymatch type of f with
+                              | list _ -> _ => unfold f in H
+                              end
+                         | [ H : context[~(exists v : ?T, ?m = @?k v) -> _] |- _ ]
+                           => rewrite (@pull_ex_not T (fun v => m = k v)) in H
+                         | [ H : context[(?A /\ ?B) -> ?C] |- _ ]
+                           => rewrite (@impl_and_l A B C) in H
+                         end
+                       | progress destruct_head'_and
+                       | progress destruct_head'_prod
+                       | progress repeat autounfold with trace_combinators in *
+                       | progress simpl in *
+                       | progress unfold Send_a in * ].
+        Local Ltac do_solve :=
+          repeat match goal with
+                 | [ H : True -> _ |- _ ] => specialize (H I)
+                 | [ H : False |- _ ] => exfalso; exact H
+                 | [ |- ?x = ?x ] => reflexivity
+                 | _ => progress destruct_head'_and
+                 | _ => progress destruct_head'_ex
+                 | _ => progress destruct_head' iff
+                 | _ => progress subst
+                 | [ H : RecieveNetwork _ = RecieveNetwork _ |- _ ]
+                   => inversion H; clear H
+                 | [ H : SendNetwork _ = SendNetwork _ |- _ ]
+                   => inversion H; clear H
+                 | [ H : Some _ = Some _ |- _ ]
+                   => inversion H; clear H
+                 | [ H : (exists v, _ = _) -> _ |- _ ]
+                   => specialize (H (ex_intro _ _ eq_refl))
+                 | [ H : _ = _ -> _ |- _ ]
+                   => specialize (H eq_refl)
+                 end.
+        induction partial_trace as [|m partial_trace IH].
+        { do_unfold; pose m_in as m_in'; destruct m_in; do_solve. }
+        { simpl @List.app in *.
+          unfold on_input_RecieveNetwork in *.
+          repeat match goal with
+                 | [ H : context[@holds_of_all_messages ?T ?P (?x :: ?xs)%list] |- _ ]
+                   => rewrite (@holds_of_all_messages_cons T P x xs) in H
+                 | [ H : context[@holds_of_all_messages ?T ?P (?ls1 ++ ?ls2)%list] |- _ ]
+                   => rewrite (@holds_of_all_messages_app T P x xs) in H
+                 end.
+          repeat first [ progress destruct_head'_prod
+                       | progress destruct_head'_and
+                       | progress destruct_head' iff ].
+          apply IH; clear IH;
+            repeat match goal with |- and _ _ => apply conj end; try assumption.
+(*          Focus 2.
+          { assumption.
+            repeat match goal with
+                   | [ H : _ = _ -> _ |- _ ] => specialize (H eq_refl)
+                   | _ => progress subst
+                   | [ H : (exists v, _ = _) -> _ |- _ ] => specialize (H (ex_intro _ _ eq_refl))
+                   | _ => progress destruct_head'_ex
+                   | [ H : Random _ = Random _ |- _ ] => inversion H; clear H
+                   | [ H : ?x = ?y -> _ |- _ ]
+                     => is_var x; destruct x
+                   end.
+          end.
+          rewrite H' in H4.
+                     (input * option pre_output)
+                     _
+                     m
+                     (partial_trace ++ (m_in, x) :: restx)%list)
+            in H4.
+          unfold holds_of_all_messages
+        { do_unfold; pose m_in as m_in'; destruct m_in; do_solve. }
+        destruct partial_trace as [|m0 [|m1 [|m2 [|m3 [|m4 partial_trace].
+        { do_unfold; pose m_in as m_in'; destruct m_in; do_solve. }
+        { destruct m0 as [m0 ?]; pose m0 as m0'; do_unfold; destruct m0; do_solve.
+          { destruct partial_trace as [|m1 partial_trace].*)
+            (*
+            { pose m_in as m_in'; destruct m_in; do_unfold; do_solve.
+        }
+        { do_unfold; pose m_in as m_in'; destruct m_in.
+
+          do_solve. }
+        { do_unfold; destruct_head' input; do_solve. }
+        { do_unfold; pose m_in as m_in'; destruct m_in; do_solve. }
+            pose m_in as m_in'; destruct m_in;
+              (*destruct_head input;*)
+
+            { repeat match goal with
+                     | [ H : ~True -> _ |- _ ] => clear H
+                     end.
+              repeat match goal with
+                         | _ => progress destruct_head'_and
+                         | [ H : (exists v, ?m = @?k v) -> _ |- _ ]
+                           => specialize (H (ex_intro _ _ eq_refl))
+                         | [ H : context[~(exists v : ?T, ?m = @?k v) -> _] |- _ ]
+                           => rewrite (@pull_ex_not T (fun v => m = k v)) in H
+                         | [ H : context[(?A /\ ?B) -> ?C] |- _ ]
+                           => rewrite (@impl_and_l A B C) in H
+                         | [ H : (exists v, ?m = @?k v) -> _ |- _ ]
+                           => first [ specialize (H (ex_intro _ m eq_refl))
+                                    | let H' := fresh in
+                                      assert (H' : forall v, m <> k v) by (clear; discriminate);
+                                      clear H H' ]
+                         | [ H : Some ?x = Some ?y -> _ |- _ ]
+                           => first [ specialize (H eq_refl)
+                                    | let H' := fresh in
+                                      assert (H' : x <> y) by (clear; discriminate);
+                                      clear H H' ]
+                         | [ H : ?A, H' : ?A -> ?B |- _ ]
+                           => specialize (H' H)
+                         | [ H : (forall v, ?m <> @?k v) -> ?P |- _ ]
+                           => let H' := fresh in
+                              first [ assert (H' : forall v, m <> k v) by (clear; discriminate);
+                                      cbv beta in H';
+                                      specialize (H H')
+                                    (*| clear H*) ]
+                         | [ H : ?x <> ?x -> _ |- _ ]
+                           => clear H
+                         | [ H : (?x <> ?y) -> ?P |- _ ]
+                           => let H' := fresh in
+                              assert (H' : x <> y) by (clear; discriminate);
+                                specialize (H H')
+                         | [ H : ?x = ?y -> ?P |- _ ]
+                           => first [ specialize (H eq_refl)
+                                    | let H' := fresh in
+                                      assert (H' : x <> y) by (clear; discriminate);
+                                      clear H H' ]
+                         | [ H : (?A -> ?B) -> ?C, H' : ?A |- _ ]
+                           => assert (B -> C) by (intro; apply H; intro; assumption);
+                                clear H
+                         | [ H : ((exists v, ?m = @?k v) -> _) -> ?P |- _ ]
+                           => assert P
+                             by (apply H; let H' := fresh in intro H'; exfalso; revert H'; apply pull_ex_not; clear; discriminate);
+                                clear H
+                         end.
+                  repeat match goal with
+                         | [ H : False |- _ ] => exfalso; exact H
+                         | [ H : context[List.Exists _ (_ :: _)] |- _ ]
+                           => rewrite List.Exists_cons in H
+                         | [ H : context[List.Exists _ nil] |- _ ]
+                           => rewrite List.Exists_nil in H
+                         | [ H : True -> _ |- _ ] => specialize (H I)
+                         | [ H : _ \/ False |- _ ] => destruct H
+                         end.
+                  unfold Send_a in *.
+              clear H95 H23.
+            Focus 2.
+              match goal with
+              end.
+              match goal with
+                   | [ H : Some ?x <> Some _ -> (True -> Random _ = ?k) /\ _ |- _ ]
+                     => is_var x; lazymatch k with Random _ => fail | _ => idtac end;
+                          destruct x
+                   | [ H : ?x <> Some _ -> (True -> Random _ = ?k) /\ _ |- _ ]
+                     => is_var x; lazymatch k with Random _ => fail | _ => idtac end;
+                          destruct x
+                   end.
+
+          { destruct_head' output.
+            { destruct_head' pre_output; try reflexivity.
+              { destruct_head' input.
+                { repeat match goal with
+                         | _ => progress destruct_head'_and
+                         | [ H : (exists v, ?m = @?k v) -> _ |- _ ]
+                           => specialize (H (ex_intro _ _ eq_refl))
+                         | [ H : context[~(exists v : ?T, ?m = @?k v) -> _] |- _ ]
+                           => rewrite (@pull_ex_not T (fun v => m = k v)) in H
+                         | [ H : context[(?A /\ ?B) -> ?C] |- _ ]
+                           => rewrite (@impl_and_l A B C) in H
+                         | [ H : (exists v, ?m = @?k v) -> _ |- _ ]
+                           => first [ specialize (H (ex_intro _ m eq_refl))
+                                    | let H' := fresh in
+                                      assert (H' : forall v, m <> k v) by (clear; discriminate);
+                                      clear H H' ]
+                         | [ H : Some ?x = Some ?y -> _ |- _ ]
+                           => first [ specialize (H eq_refl)
+                                    | let H' := fresh in
+                                      assert (H' : x <> y) by (clear; discriminate);
+                                      clear H H' ]
+                         | [ H : ?A, H' : ?A -> ?B |- _ ]
+                           => specialize (H' H)
+                         | [ H : (forall v, ?m <> @?k v) -> ?P |- _ ]
+                           => let H' := fresh in
+                              first [ assert (H' : forall v, m <> k v) by (clear; discriminate);
+                                      cbv beta in H';
+                                      specialize (H H')
+                                    (*| clear H*) ]
+                         | [ H : ?x <> ?x -> _ |- _ ]
+                           => clear H
+                         | [ H : (?x <> ?y) -> ?P |- _ ]
+                           => let H' := fresh in
+                              assert (H' : x <> y) by (clear; discriminate);
+                                specialize (H H')
+                         | [ H : ?x = ?y -> ?P |- _ ]
+                           => first [ specialize (H eq_refl)
+                                    | let H' := fresh in
+                                      assert (H' : x <> y) by (clear; discriminate);
+                                      clear H H' ]
+                         | [ H : (?A -> ?B) -> ?C, H' : ?A |- _ ]
+                           => assert (B -> C) by (intro; apply H; intro; assumption);
+                                clear H
+                         | [ H : ((exists v, ?m = @?k v) -> _) -> ?P |- _ ]
+                           => assert P
+                             by (apply H; let H' := fresh in intro H'; exfalso; revert H'; apply pull_ex_not; clear; discriminate);
+                                clear H
+                         end.
+                  repeat match goal with
+                         | [ H : False |- _ ] => exfalso; exact H
+                         | [ H : context[List.Exists _ (_ :: _)] |- _ ]
+                           => rewrite List.Exists_cons in H
+                         | [ H : context[List.Exists _ nil] |- _ ]
+                           => rewrite List.Exists_nil in H
+                         | [ H : True -> _ |- _ ] => specialize (H I)
+                         | [ H : _ \/ False |- _ ] => destruct H
+                         end.
+                  SearchAbout List.Exists.
+                  simpl in *.
+                  move H0 at bottom.
+                  repeat match goal with
+                         end.
+                  match goal with
+                  end.
+                  .
+                  intro
+                  clear H14.
+
+                  match goal with
+                  | [
+
+                  simpl in *.
+
+                  => rewrite pull_ex_not in H
+                end.
+                  => assert P; [ apply H; cut (forall v, m <> k v); clear;
+                                 [ | discriminate ]
+                               | ]
+                end.
+
+                cut (
+                  test (assert (forall v, m <> k v) by (clear; discriminate));
+
+                end.
+                clear.
+                discriminate.
+          progress simpl in *.
+        unfold unfold trace_satisfies_external_SKE_spec
+
+
+    End
+             *)
+      Abort.
+    End per_connection_choices.
+  End per_connection_parameters.
+
+  Definition synthesis_goal
+    := { state : Type
+     & { init : state -> Prop
+     & { step : _ (* state -> input -> option pre_output -> state -> Prop *)
+       | forall trace
+                (our_longterm_secret : secret),
+           exists (our_ephemeral_secret : secret)
+                  (their_ephemeral_public their_longterm_public : public),
+             @allows_behavior state input (option pre_output) init step trace
+             -> @trace_satisfies_full_SKE_spec our_longterm_secret our_ephemeral_secret their_ephemeral_public their_longterm_public trace
+         } } }.
+End spec.
